Funny/Chap3/Terms.lean
@@ -165,19 +165,12 @@ theorem structural_induction (P : T → Prop) :
   apply subterms_smaller_size
   exact hr
 
--- inductive T : Type where
---   | true : T
---   | false : T
---   | if_then_else : T → T → T → T
---   | zero : T
---   | succ : T → T
---   | pred : T → T
---   | is_zero : T → T
---   deriving DecidableEq, Ord
-
 inductive IsBool : T → Prop where
   | true : IsBool T.true
   | false : IsBool T.false
+
+def is_bool (t : T) : Prop :=
+  t = T.true ∨ t = T.false
 
 theorem IsBool.cases : ∀ {x : T}, IsBool x → x = T.true ∨ x = T.false := by
   intro x is_b
@@ -187,6 +180,9 @@ inductive IsNumber : T → Prop where
   | zero : IsNumber T.zero
   | succ : ∀ {n}, {_ : IsNumber n} → IsNumber (T.succ n)
 
+def is_number (t : T) : Prop :=
+  t = T.zero ∨ ∃ n, t = T.succ n
+
 theorem IsNumber.cases : ∀ {x : T}, IsNumber x → x = T.zero ∨ ∃n, IsNumber n ∧ x = T.succ n := by
   intro x is_n
   cases is_n <;> simp; assumption
@@ -195,15 +191,251 @@ inductive IsValue : T → Prop where
   | bool : ∀ {t}, {_ : IsBool t} → IsValue t
   | number : ∀ {n}, {_ : IsNumber n} → IsValue n
 
+theorem IsValue.cases : ∀ {x : T}, IsValue x →
+  (x = T.true ∨ x = T.false) ∨ (x = T.zero ∨ ∃ n : T, IsNumber n ∧ x = T.succ n) := by
+  intro x is_value
+  cases is_value with
+  | @bool is_bool => left; exact is_bool.cases
+  | @number is_number => right; exact is_number.cases
+
 open T in
 inductive Eval : Rel T T where
   | if_true : ∀ {t₂ t₃}, Eval (if_then_else true t₂ t₃) t₂
   | if_false : ∀ {t₂ t₃}, Eval (if_then_else false t₂ t₃) t₃
-  | if : ∀ {t₁ t₁' t₂ t₃}, Eval t₁ t₁' → Eval (if_then_else t₁ t₂ t₃) (if_then_else t₁' t₂ t₃)
+  | if_ : ∀ {t₁ t₁' t₂ t₃}, Eval t₁ t₁' → Eval (if_then_else t₁ t₂ t₃) (if_then_else t₁' t₂ t₃)
   | succ : ∀ {t t'}, Eval t t' → Eval (succ t) (succ t')
   | pred_zero : Eval (pred zero) zero
   | pred_succ : ∀ {t}, {_ : IsNumber t} → Eval (pred (succ t)) t
   | pred : ∀ {t t'}, Eval t t' → Eval (pred t) (pred t')
   | is_zero_zero : Eval (is_zero zero) true
   | is_zero_succ : ∀ {t}, {_ : IsNumber t} → Eval (is_zero (succ t)) false
-  | is_zero : ∀ {t t'}, Eval t t' → Eval t t' → Eval (is_zero t) (is_zero t')
+  | is_zero : ∀ {t t'}, Eval t t' → Eval (is_zero t) (is_zero t')
+
+@[simp]
+def is_normal_form (x : T) : Prop := ¬∃y : T, Eval x y
+
+@[simp]
+def is_stuck (x : T) : Prop := is_normal_form x ∧ ¬IsValue x
+
+theorem succ_is_not_zero : ∀ {t₁ t₂}, Eval (T.succ t₁) t₂ → ¬(t₂ = T.zero) := by
+  intro t₁ t₂ ev₁ eq
+  rw [eq] at ev₁
+  cases ev₁
+
+theorem booleans_do_not_eval : ∀ (x : T), {_ : IsBool x} → is_normal_form x := by
+  intro x is_bool ⟨y, ev⟩
+  have := is_bool.cases
+  cases x with
+  | true
+  | false => cases ev
+  | is_zero
+  | pred
+  | if_then_else
+  | zero
+  | succ =>
+    simp_all
+
+theorem numbers_do_not_eval : ∀ (x : T), {_ : IsNumber x} → is_normal_form x := by
+  intro x is_number ⟨y, ev⟩
+  have := is_number.cases
+  cases x with
+  | true
+  | false
+  | is_zero
+  | pred
+  | if_then_else => simp_all
+  | zero => cases ev
+  | succ m =>
+    if h : IsNumber m
+    then
+      cases ev with
+      | succ ev₁ =>
+        have := @numbers_do_not_eval m h
+        apply this ⟨ _, ev₁ ⟩
+    else
+      simp_all
+
+theorem value_implies_bool_or_number : ∀ x, IsValue x → IsBool x ∨ IsNumber x := by
+  intro x is_value
+  cases is_value with
+  | @bool x => left; assumption
+  | @number x => right; assumption
+
+theorem values_do_not_eval : ∀ (x : T), {_ : IsValue x} → is_normal_form x := by
+  intro x is_value
+  have := is_value.cases
+  if h₁ : IsNumber x then
+    exact @numbers_do_not_eval x h₁
+  else if h₂ : IsBool x then
+    exact @booleans_do_not_eval x h₂
+  else
+    have := value_implies_bool_or_number x is_value
+    cases this with
+    | inl | inr => contradiction
+
+theorem determinancy_of_one_step : ∀ {t t' t''}, (Eval t t') → (Eval t t'') → t' = t'' := by
+   intro t t' t'' ev₁ ev₂
+   cases t with
+   | true
+   | false
+   | zero => cases ev₁
+   | succ n =>
+     cases ev₁ with
+     | succ ev₃ =>
+       cases ev₂ with
+       | succ ev₄ =>
+         have := determinancy_of_one_step ev₃ ev₄
+         rw [this]
+   | pred n =>
+     cases ev₁ with
+     | pred ev₃ =>
+       cases ev₂ with
+       | pred ev₄ =>
+         have := determinancy_of_one_step ev₃ ev₄
+         rw [this]
+       | @pred_succ _ is_number =>
+         have := @IsNumber.succ t'' is_number
+         have := @numbers_do_not_eval _ this
+         exfalso
+         exact this ⟨_, ev₃⟩
+       | pred_zero => contradiction
+     | pred_zero =>
+       cases ev₂ with
+       | pred => contradiction
+       | pred_zero => rfl
+     | @pred_succ _ is_number =>
+       cases ev₂ with
+       | @pred t₃ t₄ ev₃ =>
+         have := @IsNumber.succ _ is_number
+         have := @numbers_do_not_eval _ this
+         exfalso
+         exact this ⟨_, ev₃⟩
+       | pred_succ => rfl
+   | is_zero n =>
+     cases ev₁ with
+     | is_zero_zero =>
+       cases ev₂ with
+       | is_zero_zero => rfl
+       | is_zero ev₃ =>
+         have := @IsNumber.zero
+         have := @numbers_do_not_eval _ this
+         exfalso
+         exact this ⟨_, ev₃⟩
+     | @is_zero_succ _ is_number =>
+       cases ev₂ with
+       | is_zero ev₃ =>
+         have := @IsNumber.succ _ is_number
+         exfalso
+         exact @numbers_do_not_eval _ this ⟨_, ev₃⟩
+       | is_zero_succ => rfl
+     | is_zero ev₃ =>
+       cases ev₂ with
+       | is_zero ev₄ =>
+         have := determinancy_of_one_step ev₃ ev₄
+         rw [this]
+       | @is_zero_succ _ is_number =>
+         have := @IsNumber.succ _ is_number
+         exfalso
+         exact @numbers_do_not_eval _ this ⟨_, ev₃⟩
+       | is_zero_zero =>
+         have := @IsNumber.zero
+         exfalso
+         exact @numbers_do_not_eval _ this ⟨_, ev₃⟩
+   | if_then_else x y z =>
+     cases ev₁ with
+     | if_ ev₃ =>
+       cases ev₂ with
+       | if_ ev₄ =>
+         have := determinancy_of_one_step ev₃ ev₄
+         rw [this]
+       | if_false =>
+         have := @IsBool.false
+         exfalso
+         exact @booleans_do_not_eval _ this ⟨_, ev₃⟩
+       | if_true =>
+         have := @IsBool.true
+         exfalso
+         exact @booleans_do_not_eval _ this ⟨_, ev₃⟩
+     | if_true =>
+       cases ev₂ with
+       | if_ ev₃ =>
+         have := @IsBool.true
+         exfalso
+         exact @booleans_do_not_eval _ this ⟨_, ev₃⟩
+       | if_true => rfl
+     | if_false =>
+       cases ev₂ with
+       | if_ ev₃ =>
+         have := @IsBool.false
+         exfalso
+         exact @booleans_do_not_eval _ this ⟨_, ev₃⟩
+       | if_false => rfl
+
+inductive MultiStep : Rel T T where
+  | rfl : ∀ {x}, MultiStep x x
+  | single : ∀ {x y}, Eval x y → MultiStep x y
+  | trans : ∀ {x y z}, MultiStep x y → MultiStep y z → MultiStep x z
+
+infixl:50 "⇒" => MultiStep
+
+theorem normal_form_only_eval_to_itself : ∀ x y, is_normal_form x → MultiStep x y → x = y := by
+  intro x y nfx mse
+  induction mse with
+  | rfl =>
+    rfl
+  | single ev =>
+    simp at nfx
+    exfalso
+    exact nfx _ ev
+  | trans mse₁ mse₂ ih₁ ih₂ =>
+    have eq₁ := ih₁ nfx
+    rw [eq₁] at nfx
+    have eq₂ := ih₂ nfx
+    rw [eq₁, eq₂]
+
+-- theorem uniqueness_of_normal_forms : ∀ t u u', is_normal_form u → is_normal_form u' → t ⇒ u → t ⇒ u' → u = u' := by
+--   intro t u u' nfu nfu' mse mse'
+--   induction mse with
+--   | rfl =>
+--     cases mse' with
+--     | rfl => rfl
+--     | single ev =>
+--       simp at nfu
+--       exfalso
+--       exact nfu u' ev
+--     | trans h₁ h₂ =>
+--       have x_eq_y := normal_form_only_eval_to_itself _ _ nfu h₁
+--       rw [x_eq_y] at nfu
+--       have y_eq_u := normal_form_only_eval_to_itself _ u' nfu h₂
+--       rw [x_eq_y, y_eq_u]
+--   | single ev =>
+--     cases mse' with
+--     | rfl =>
+--       simp at nfu'
+--       exfalso
+--       exact nfu' _ ev
+--     | single ev₁ =>
+--       exact determinancy_of_one_step ev ev₁
+--     | trans h₁ h₂ =>
+--       have x_ev_y := MultiStep.single ev
+--       have x_ev_u' := MultiStep.trans h₁ h₂
+--       have y_ev_u' := helper x_ev_u' x_ev_y nfu'
+--       exact helper₂ _ u' nfu y_ev_u'
+
+--   | trans h₁ h₂ ih₁ ih₂ =>
+--     cases mse' with
+--     | rfl =>
+--       have u'_eq_y := normal_form_only_eval_to_itself u' _ nfu' h₁
+--       rw [u'_eq_y] at ih₂
+--       have  z_eq_y := ih₂ nfu MultiStep.rfl u_value
+--       rw [z_eq_y, u'_eq_y]
+--     | single ev₁ =>
+--       have x_ev_u' := MultiStep.single ev₁
+--       suffices ∀ {x y z}, x ⇒ y → x ⇒ z → is_normal_form y → z ⇒ y by
+--         have y_ev_u' := this x_ev_u' h₁ nfu'
+--         exact ih₂ nfu y_ev_u' u_value
+--       exact helper
+--     | trans h₃ h₄ =>
+--       have x_ev_u' := MultiStep.trans h₃ h₄
+--       have y_ev_u' := helper x_ev_u' h₁ nfu'
+--       exact ih₂ nfu y_ev_u' u_value
