Funny/Chap3.lean
@@ -1,2 +1,0 @@
-import Chap3.Booleans
-import Chap3.Terms
