Main.lean
@@ -1,5 +1,4 @@
 import Funny
-import Funny.Chap3
 
 def main : IO Unit :=
   IO.println s!"Hello, I ran!"
